



Probability and Stochastic Processes

Lecture 20: Transformations (Part 2)

Karthik P. N.

Assistant Professor, Department of AI

Email: pnkarthik@ai.iith.ac.in

17 October 2025



Sums of Random Variables

Let X and Y be random variables.

- Show that $X + Y$ is a random variable.
- In the cases when X and Y are jointly discrete/continuous, derive the PMF/PDF of $X + Y$.
- Simplify the PMF/PDF when X and Y are independent.

Showing that $X + Y$ is a Random Variable

For any $x \in \mathbb{R}$,

$$\begin{aligned}\{X + Y < x\} &= \{X < x - Y\} \\ &= \left\{ \exists q \in \mathbb{Q} : X < q < x - Y \right\} \\ &= \bigcup_{q \in \mathbb{Q}} \{X < q, q < x - Y\} \\ &= \bigcup_{q \in \mathbb{Q}} \{X < q\} \cap \{Y < x - q\} \in \mathcal{F}\end{aligned}$$

PMF of $X + Y$ for Jointly Discrete X, Y

- X, Y jointly discrete $\implies X$ discrete, Y discrete $\implies X + Y$ discrete
- There exists countable $E \subset \mathbb{R}^2$ such that $\mathbb{P}_{X,Y}(E) = 1$
- Extract sets $E_1, E_2 \subset \mathbb{R}$ such that

$$E_1 = \{x \in \mathbb{R} : \exists y \in \mathbb{R} \text{ such that } (x, y) \in E\}, \quad \mathbb{P}_X(E_1) = 1,$$

$$E_2 = \{y \in \mathbb{R} : \exists x \in \mathbb{R} \text{ such that } (x, y) \in E\}, \quad \mathbb{P}_Y(E_2) = 1$$

- PMF of $Z = X + Y$: for any $z \in \mathbb{R}$,

$$p_Z(z) = \mathbb{P}(\{Z = z\}) = \mathbb{P}(\{X + Y = z\}) = \mathbb{P}_{X+Y}(\{z\}) = \mathbb{P}_{X,Y}\left(\underbrace{\{(x, y) : x + y = z\}}_B\right)$$

$$= \sum_{(x,y) \in B \cap E} p_{X,Y}(x, y) = \sum_{\substack{(x,y) \in E: \\ x+y=z}} p_{X,Y}(x, y) = \sum_{\substack{(x,y) \in E: \\ x+y=z}} p_{X,Y}(x, z-x) = \sum_{\substack{x: x \in E_1, \\ z-x \in E_2}} p_{X,Y}(x, z-x)$$

$$\stackrel{X \perp\!\!\!\perp Y}{=} \sum_{\substack{x: x \in E_1, \\ z-x \in E_2}} p_X(x) p_Y(z-x) = p_X * p_Y(z)$$

Sum of Two Independent Poissons

Let $X \sim \text{Poisson}(\lambda_1)$ and $Y \sim \text{Poisson}(\lambda_2)$. Assume $X \perp\!\!\!\perp Y$. Determine the distribution of $Z = X + Y$.

- Here, the sets $E \subset \mathbb{R}^2$ and $E_1, E_2 \subset \mathbb{R}$ are as follows:

$$E = \mathbb{W} \times \mathbb{W}, \quad E_1 = \mathbb{W}, \quad E_2 = \mathbb{W},$$

where $\mathbb{W} = \mathbb{N} \cup \{0\}$

- For any $z \in \mathbb{W}$,

$$\begin{aligned} p_Z(z) &= \sum_{\substack{x: x \in \mathbb{W}, \\ z-x \in \mathbb{W}}} p_X(x) p_Y(z-x) = \sum_{x=0}^z e^{-\lambda_1} \frac{\lambda_1^x}{x!} e^{-\lambda_2} \frac{\lambda_2^{z-x}}{(z-x)!} \\ &= \frac{e^{-(\lambda_1+\lambda_2)}}{z!} \sum_{x=0}^z \frac{z!}{x! (z-x)!} \lambda_1^x \lambda_2^{z-x} = e^{-(\lambda_1+\lambda_2)} \frac{(\lambda_1 + \lambda_2)^z}{z!} \end{aligned}$$

PDF of $X + Y$ for Jointly Continuous X, Y

- X, Y jointly continuous $\implies X$ continuous, Y continuous $\implies X + Y$ continuous
- CDF of $Z = X + Y$: for any $z \in \mathbb{R}$,

$$\begin{aligned}
 F_Z(z) &= \mathbb{P}(\{Z \leq z\}) = \mathbb{P}(\{X + Y \leq z\}) = \mathbb{P}_{X+Y}((-\infty, z]) = \mathbb{P}_{X,Y}(\underbrace{\{(x, y) : x + y \leq z\}}_B) \\
 &= \iint_B f_{X,Y}(u, v) \, dv \, du = \int_{-\infty}^{\infty} \int_{-\infty}^{z-u} f_{X,Y}(u, v) \, dv \, du \stackrel{t=u+v}{=} \int_{-\infty}^{\infty} \int_{-\infty}^z f_{X,Y}(u, t-u) \, dt \, du \\
 &= \int_{-\infty}^z \underbrace{\int_{-\infty}^{\infty} f_{X,Y}(u, t-u) \, du}_{g(t)} \, dt
 \end{aligned}$$

- Thus, it follows that the PDF of Z is given by

$$\forall z \in \mathbb{R}, \quad f_Z(z) = g(z) = \int_{-\infty}^{\infty} f_{X,Y}(u, z-u) \, du \stackrel{X \perp Y}{=} \int_{-\infty}^{\infty} f_X(u) f_Y(z-u) \, du = f_X * f_Y(z)$$

Sum of Two Independent Exponentials

Let $X \sim \text{Exponential}(\mu_1)$ and $Y \sim \text{Exponential}(\mu_2)$. Assume $X \perp\!\!\!\perp Y$. Determine the PDF of $Z = X + Y$.

- For any $z \in (0, +\infty)$,

$$f_Z(z) = \int_{-\infty}^{\infty} f_X(u) f_Y(z-u) du = \int_0^{\infty} \mu_1 e^{-\mu_1 u} f_Y(z-u) du = \int_0^z \mu_1 e^{-\mu_1 u} \mu_2 e^{-\mu_2 (z-u)} du$$

$$= \mu_1 \mu_2 e^{-\mu_2 z} \int_0^z e^{(\mu_2 - \mu_1) u} du = \begin{cases} \underbrace{\mu^2 z e^{-\mu z}}_{\text{Erlang}(2)}, & \mu_1 = \mu_2 = \mu, \\ \frac{\mu_1 \mu_2}{\mu_2 - \mu_1} (e^{-\mu_1 z} - e^{-\mu_2 z}), & \mu_1 \neq \mu_2. \end{cases}$$

Functions of Independent Random Variables are Independent Random Variables

Let X and Y be two random variables. Let $g : \mathbb{R} \rightarrow \mathbb{R}$ and $h : \mathbb{R} \rightarrow \mathbb{R}$ be **measurable**. Show that

$$X \perp\!\!\!\perp Y \implies g(X) \perp\!\!\!\perp h(Y).$$

For any $B_1, B_2 \in \mathcal{B}(\mathbb{R})$,

$$\begin{aligned} P_{g(X), h(Y)}(B_1 \times B_2) &= \mathbb{P}\left(\{g(X) \in B_1\} \cap \{h(Y) \in B_2\}\right) \\ &= \mathbb{P}\left(\{X \in g^{-1}(B_1)\} \cap \{Y \in h^{-1}(B_2)\}\right) = \mathbb{P}_{X,Y}(g^{-1}(B_1) \times h^{-1}(B_2)) \\ &\stackrel{X \perp\!\!\!\perp Y}{=} \mathbb{P}_X(g^{-1}(B_1)) \cdot \mathbb{P}_Y(h^{-1}(B_2)) = \mathbb{P}_{g(X)}(B_1) \cdot \mathbb{P}_{h(Y)}(B_2). \end{aligned}$$

Sum of Random Number of Random Variables

Let $\{X_1, X_2, \dots\}$ be a countably infinite collection of **IID** random variables having a common CDF F .

Let N be a discrete random variable taking values in natural numbers and having PMF p_N .

Let N be **independent** of $\{X_i : i \in \mathbb{N}\}$.

Consider the sum

$$S_N := \sum_{i=1}^N X_i; \quad S_N(\omega) = \sum_{i=1}^{N(\omega)} X_i(\omega), \quad \omega \in \Omega.$$

- Show that $S_N : \Omega \rightarrow \mathbb{R}$ is a random variable with respect to \mathcal{F} .
- Determine the CDF of S_N .

Showing that S_N is a Random Variable

- Let us define sets

$$E_n := \{N = n\}, \quad n \in \mathbb{N}.$$

- Then, $\{E_n\}$ forms a partition of Ω , i.e.,

$$\Omega = \bigsqcup_{n \in \mathbb{N}} E_n.$$

- For any $x \in \mathbb{R}$,

$$\{S_N \leq x\} = \bigsqcup_{n \in \mathbb{N}} \left(\{S_N \leq x\} \cap E_n \right) = \bigsqcup_{n \in \mathbb{N}} \left(\{S_N \leq x\} \cap \{N = n\} \right) = \bigsqcup_{n \in \mathbb{N}} \left(\{S_n \leq x\} \cap \{N = n\} \right) \in \mathcal{F}.$$

CDF of S_N

- For any $x \in \mathbb{R}$,

$$\begin{aligned} F_{S_N}(x) &= \mathbb{P}(\{S_N \leq x\}) = \sum_{n \in \mathbb{N}} \mathbb{P}(\{S_N \leq x\} \cap E_n) = \sum_{n \in \mathbb{N}} \mathbb{P}(\{S_N \leq x\} \cap \{N = n\}) \\ &= \sum_{n \in \mathbb{N}} \mathbb{P}(\{S_n \leq x\} \cap \{N = n\}) = \sum_{n \in \mathbb{N}} \mathbb{P}(\{S_n \leq x\}) \cdot \mathbb{P}(\{N = n\}) \\ &= \sum_{n \in \mathbb{N}} \mathbb{P}(\{S_n \leq x\}) \cdot p_N(n). \end{aligned}$$

Sum of Geometrically Many Exponential RVs

Evaluate the CDF of S_N for the case when $X_1, X_2, \dots \stackrel{\text{i.i.d.}}{\sim} \text{Exp}(\lambda)$ and $N \sim \text{Geom}(p)$, with $N \perp\!\!\!\perp \{X_1, X_2, \dots\}$.

- The sum S_n of n IID exponentials follows $\text{Erlang}(n)$ distribution with PDF

$$f_{S_n}(x) = \frac{\lambda^n x^{n-1} e^{-\lambda x}}{(n-1)!}, \quad x \geq 0.$$

- CDF of S_N :

$$\begin{aligned} F_{S_N}(x) &= \sum_{n \in \mathbb{N}} \mathbb{P}(\{S_n \leq x\}) \cdot p_N(n) \\ &= \sum_{n \in \mathbb{N}} \left(\int_0^x \frac{\lambda^n u^{n-1} e^{-\lambda u}}{(n-1)!} du \right) \cdot p(1-p)^{n-1} \\ &= \begin{cases} 1 - e^{-p\lambda x}, & x \geq 0, \\ 0, & x < 0. \end{cases} \end{aligned}$$

Thus, $S_N \sim \text{Exponential}(p\lambda)$

General Transformations and the Jacobian Formula

General Transformations

Fix $(\Omega, \mathcal{F}, \mathbb{P})$.

Let $X : \Omega \rightarrow \mathbb{R}$ be a continuous random variable with PDF f_X .

Given $g : \mathbb{R} \rightarrow \mathbb{R}$ that is **monotone** and **differentiable** with non-zero derivative throughout its domain, what is the PDF of $Y = g(X)$?

General Transformations

Fix $(\Omega, \mathcal{F}, \mathbb{P})$.

Let $X : \Omega \rightarrow \mathbb{R}$ be a continuous random variable with PDF f_X .

Given $g : \mathbb{R} \rightarrow \mathbb{R}$ that is **monotone** and **differentiable** with non-zero derivative throughout its domain, what is the PDF of $Y = g(X)$?

Note that g admits an inverse, say g^{-1} .

General Transformations: g Monotone Increasing

$$\begin{aligned}F_Y(y) &= \mathbb{P}(\{Y \leq y\}) \\&= \mathbb{P}(\{g(X) \leq y\}) \\&= \mathbb{P}(\{X \leq g^{-1}(y)\}) \\&= \int_{-\infty}^{g^{-1}(y)} f_X(u) \, du\end{aligned}$$

make substitution $g(u) = v$

$$= \int_{-\infty}^y \underbrace{\frac{f_X(g^{-1}(v))}{g'(g^{-1}(v)))}}_{f_Y(v)} \, dv$$

Thus, we have

$$f_Y(y) = \begin{cases} \frac{f_X(g^{-1}(y))}{g'(g^{-1}(y))}, & y \in \text{Range}(g), \\ 0, & y \notin \text{Range}(g). \end{cases}$$

General Transformations: g Monotone Decreasing

$$\begin{aligned}F_Y(y) &= \mathbb{P}(\{Y \leq y\}) \\&= \mathbb{P}(\{g(X) \leq y\}) \\&= \mathbb{P}(\{X \geq g^{-1}(y)\}) \\&= \int_{g^{-1}(y)}^{+\infty} f_X(u) \, du \\&= \int_y^{\infty} \frac{f_X(g^{-1}(v))}{g'(g^{-1}(v))} \, dv\end{aligned}$$

make substitution $g(u) = v$

General Transformations: g Monotone Decreasing

$$\begin{aligned}F_Y(y) &= \mathbb{P}(\{Y \leq y\}) \\&= \mathbb{P}(\{g(X) \leq y\}) \\&= \mathbb{P}(\{X \geq g^{-1}(y)\}) \\&= \int_{g^{-1}(y)}^{+\infty} f_X(u) \, du \\&= \int_y^{\infty} \frac{f_X(g^{-1}(v))}{g'(g^{-1}(v))} \, dv\end{aligned}$$

make substitution $g(u) = v$

It thus follows that

$$f_Y(y) = \begin{cases} \frac{f_X(g^{-1}(y))}{-g'(g^{-1}(y))}, & y \in \text{Range}(g), \\ 0, & y \notin \text{Range}(g). \end{cases}$$

General Transformations: g Monotone, Differentiable

When g is **monotone and differentiable** throughout its domain:

$$Y = g(X), \quad f_Y(y) = \begin{cases} \frac{f_X(g^{-1}(y))}{|g'(g^{-1}(y))|}, & y \in \text{Range}(g), \\ 0, & y \notin \text{Range}(g). \end{cases}$$